Sbackend correctness statement sketch

stanfrontend/CStan.v
@@ -607,3 +607,6 @@ Definition semantics_transformed_parameters (p: program) (m: mem) :=
 						      
 Definition semantics_generated_quantities (p: program) (m: mem) :=
   semantics_gen p m p.(prog_generated_quantities).
+
+Definition semantics (p: program) (m: mem) :=
+  semantics_gen p m p.(prog_model).
