stanfrontend/Sbackendproof.v
@@ -1,0 +1,29 @@
+Require Import Smallstep.
+Require Import Sbackend.
+Require Import CStan.
+Require Import Clight.
+Require Import Ssemantics.
+Require Import Errors.
+Require Import Globalenvs.
+Require Import Memory.
+
+
+Section PRESERVATION.
+
+Variable prog: CStan.program.
+Variable tprog: Clight.program.
+Variable m0: mem.
+Hypothesis TRANSF: Sbackend.backend prog = OK tprog.
+Hypothesis INITMEM: Genv.init_mem prog = Some m0.
+Let ge := CStan.globalenv prog.
+Let tge := globalenv tprog.
+
+Check Clight.semantics1.
+Check CStan.semantics.
+
+Theorem transf_program_correct:
+  forward_simulation (CStan.semantics prog m0) (Clight.semantics1 tprog).
+Admitted.
+
+End PRESERVATION.
+
